howeScript.sml
@@ -1,0 +1,177 @@
+(*
+   This file formalises Howe's method following the description of
+   Pitts 2011 chapter "Howe's method for higher-order languages".
+*)
+open HolKernel Parse boolLib bossLib term_tactic;
+open expTheory valueTheory arithmeticTheory listTheory stringTheory alistTheory
+     optionTheory pairTheory ltreeTheory llistTheory bagTheory pure_langTheory
+     pred_setTheory;
+
+val _ = new_theory "howe";
+
+
+(* -- basics -- *)
+
+(* the set of all values with at most free variables vars *)
+Definition Vals_def:
+  Vals vars = { v | freevars_v v ⊆ set vars }
+End
+
+(* the set of all expressions with at most free variables vars *)
+Definition Exps_def:
+  Exps vars = { e | set (freevars e) ⊆ set vars }
+End
+
+Theorem Exps_EMPTY_closed[simp]:
+  e IN Exps [] ⇔ closed e
+Proof
+  fs [Exps_def,closed_def]
+QED
+
+
+(* -- applicative (bi)similarity -- *)
+
+Definition unfold_rel_def:
+  unfold_rel rel (e1, e2) ⇔
+    closed e1 ∧ closed e2 ∧
+    (* this follows the paper directly *)
+    ∀x e1'. eval e1 = Closure x e1' ⇒
+            ∃e2'. eval e2 = Closure x e2' ∧
+                  ∀e. closed e ⇒ rel (subst x e e1', subst x e e2')
+    (* but I think we need one such conjunct for each result alternative *)
+End
+
+Definition app_simulation_def:
+  app_simulation S ⇔
+    ∀e1 e2. S (e1, e2) ⇒ unfold_rel S (e1, e2)
+End
+
+Definition opp_def:
+  opp s (x,y) ⇔ (y,x) IN s
+End
+
+Definition app_bisimulation_def:
+  app_bisimulation S ⇔ app_simulation S ∧ app_simulation (opp S)
+End
+
+Definition FF_def:
+  FF s = { (e1, e2) | unfold_rel s (e1, e2) }
+End
+
+Triviality monotone_similarity:
+  monotone FF
+Proof
+  fs [fixedPointTheory.monotone_def,FF_def,unfold_rel_def]
+  \\ fs [SUBSET_DEF,FORALL_PROD,IN_DEF]
+  \\ metis_tac []
+QED
+
+Definition app_similarity_def:
+  app_similarity = gfp FF
+End
+
+val _ = set_fixity "≲" (Infixl 480);
+Overload "≲" = “λx y. app_similarity (x,y)”;
+
+Theorem app_similarity_thm =
+  MATCH_MP fixedPointTheory.gfp_greatest_fixedpoint monotone_similarity
+  |> SIMP_RULE std_ss [GSYM app_similarity_def]
+
+Theorem app_similarity_iff = (* result (5.4) *)
+  app_similarity_thm |> CONJUNCT1 |> GSYM
+    |> SIMP_RULE std_ss [FF_def,EXTENSION,FORALL_PROD,GSPECIFICATION,EXISTS_PROD]
+    |> SIMP_RULE std_ss [IN_DEF];
+
+Theorem app_simulation_SUBSET_app_similarity:
+  app_simulation R ⇒ R ⊆ app_similarity
+Proof
+  rw [app_similarity_def,app_simulation_def]
+  \\ fs [fixedPointTheory.gfp_def,SUBSET_DEF,FORALL_PROD]
+  \\ fs [IN_DEF,FF_def,EXISTS_PROD] \\ metis_tac []
+QED
+
+Theorem app_simulation_app_similarity:
+  app_simulation app_similarity
+Proof
+  fs [app_simulation_def]
+  \\ assume_tac app_similarity_iff
+  \\ metis_tac []
+QED
+
+Triviality monotone_bisimilarity:
+  monotone (λs. { (e1,e2) | (e1,e2) IN FF s ∧ (e2,e1) IN FF (opp s) })
+Proof
+  fs [fixedPointTheory.monotone_def,FF_def,unfold_rel_def,opp_def]
+  \\ fs [SUBSET_DEF,FORALL_PROD,IN_DEF,opp_def]
+  \\ metis_tac []
+QED
+
+Definition app_bisimilarity_def:
+  app_bisimilarity = gfp (λs. { (e1,e2) | (e1,e2) IN FF s ∧ (e2,e1) IN FF (opp s) })
+End
+
+val _ = set_fixity "≃" (Infixl 480);
+Overload "≃" = “λx y. app_bisimilarity (x,y)”;
+
+Theorem app_bisimilarity_thm =
+  MATCH_MP fixedPointTheory.gfp_greatest_fixedpoint monotone_bisimilarity
+  |> SIMP_RULE std_ss [GSYM app_bisimilarity_def]
+
+Theorem app_bisimilarity_iff = (* result (5.5) *)
+  app_bisimilarity_thm |> CONJUNCT1 |> GSYM
+    |> SIMP_RULE std_ss [FF_def,EXTENSION,FORALL_PROD,GSPECIFICATION,EXISTS_PROD]
+    |> SIMP_RULE (std_ss++boolSimps.CONJ_ss) [IN_DEF,unfold_rel_def,opp_def]
+    |> REWRITE_RULE [GSYM CONJ_ASSOC];
+
+Theorem app_bisimulation_SUBSET_app_bisimilarity:
+  app_bisimulation R ⇒ R ⊆ app_bisimilarity
+Proof
+  rw [app_bisimilarity_def,app_bisimulation_def,app_simulation_def]
+  \\ fs [fixedPointTheory.gfp_def,SUBSET_DEF,FORALL_PROD,opp_def,IN_DEF]
+  \\ fs [IN_DEF,FF_def,EXISTS_PROD,unfold_rel_def,opp_def]
+  \\ rw [] \\ qexists_tac ‘R’ \\ rw []
+  \\ res_tac \\ fs []
+QED
+
+Theorem app_bisimulation_app_bisimilarity:
+  app_bisimulation app_bisimilarity
+Proof
+  fs [app_bisimulation_def,app_simulation_def,opp_def,IN_DEF,unfold_rel_def]
+  \\ assume_tac app_bisimilarity_iff
+  \\ metis_tac [unfold_rel_def]
+QED
+
+Theorem PreOrder_app_similarity: (* exercise (5.3.3) *)
+  PreOrder $≲
+  (* hrmm, the statement isn't right because it needs to be
+     restricted to consider only closed expressions *)
+Proof
+  cheat
+QED
+
+Theorem equivalence_app_bisimilarity: (* exercise (5.3.3) *)
+  equivalence $≃
+  (* hrmm, the statement isn't right because it needs to be
+     restricted to consider only closed expressions *)
+Proof
+  cheat
+QED
+
+Theorem app_bisimilarity_similarity: (* prop (5.3.4) *)
+  e1 ≃ e2 ⇔ e1 ≲ e2 ∧ e2 ≲ e1
+Proof
+  cheat
+QED
+
+
+(* -- congruence -- *)
+
+
+(* -- Howe's construction -- *)
+
+
+(* -- contextual equivalence -- *)
+
+
+
+val _ = export_theory();
